Redefine in terms of finsets

src/DFA.lean
@@ -8,11 +8,17 @@ structure DFA (alphabet : Type u) :=
 [alphabet_fintype : fintype alphabet]
 (state : Type v)
 [state_fintype : fintype state]
+[state_dec : decidable_eq state]
 (step : state → alphabet → state)
 (start : state)
-(accept_states : set state)
+(accept_states : finset state)
 
 namespace DFA
+
+instance dec (M : DFA α) := M.state_dec
+
+instance fin₁ (M : DFA α) := M.alphabet_fintype
+instance fin₂ (M : DFA α) := M.state_fintype
 
 def eval (M : DFA α) : list α → M.state :=
 list.foldl M.step M.start
